compiler/backend/semantics/labPropsScript.sml
@@ -635,4 +635,15 @@ val _ = export_rewrites["sec_ok_pre_def"];
 val _ = overload_on("all_enc_ok_pre",``λc ls.
   EVERY (sec_ok_pre c) ls``);
 
+(* invariant: labels have correct section number and are non-zero *)
+
+val sec_label_ok_def = Define`
+  (sec_label_ok k (Label l1 l2 len) ⇔ l1 = k ∧ l2 ≠ 0) ∧
+  (sec_label_ok _ _ = T)`;
+val _ = export_rewrites["sec_label_ok_def"];
+
+val sec_labels_ok_def = Define`
+  sec_labels_ok (Section k ls) ⇔ EVERY (sec_label_ok k) ls`;
+val _ = export_rewrites["sec_labels_ok_def"];
+
 val _ = export_theory();
